\documentclass[11pt]{article}

\newcommand{\titrechapitre}{}%Ensembles de nombres -- Exercices}
\newcommand{\titreclasse}{}%Lycée Jean-Baptiste \textsc{Corot}}
\newcommand{\pagination}{}%\thepage/\pageref{LastPage}}
\newcommand{\topbotmargins}{1cm}
\newcommand{\spacebelowexo}{2mm}
\input{/home/erou/teaching/corot/latex/layout-color.tex}

\begin{document}

\begin{exo}[Produits]
  Pour chacune des fonctions suivantes, donner l'expression de la dérivée.
  \begin{align*}
    \textbf{a)}\;& f:x\mapsto (x-1)\sqrt x &
    \textbf{b)}\;& g:x\mapsto (x^2-x)\left( 1+\frac{1}{x^2} \right) &
    \textbf{c)}\;& h:x\mapsto (\sqrt x + x^2)\left( \frac{1}{x}+\frac{1}{x^2} \right)
  \end{align*}
\end{exo}

\begin{exo}[Quotients]
  Pour chacune des fonctions suivantes, donner l'expression de la dérivée.
  \begin{align*}
    \textbf{a)}\;& f:x\mapsto \frac{1+x^4}{x+1} &
    \textbf{b)}\;& g:x\mapsto \frac{1-x}{1+\sqrt x} &
    \textbf{c)}\;& h:x\mapsto \frac{1-x^3}{1-x}
  \end{align*}
\end{exo}

\begin{exo}[Compositions]
  Pour chacune des fonctions suivantes, donner l'expression de la dérivée.
  \begin{align*}
    \textbf{a)}\;& f:x\mapsto \sqrt{2x+1} &
    \textbf{b)}\;& g:x\mapsto (5x+1)^{11} &
    \textbf{c)}\;& h:x\mapsto \frac{1}{(3x+2)^7}
  \end{align*}
\end{exo}

\begin{exo}[Un peu de tout, $\star$]
  Pour chacune des fonctions suivantes, donner l'expression de la dérivée.
  \begin{align*}
    \textbf{a)}\;& f:x\mapsto 2x^3\sqrt{x} &
    \textbf{b)}\;& g:x\mapsto 3(3x+3)^3+3 &
    \textbf{c)}\;& h:x\mapsto 3(3x^3+3)+3 \\
    \textbf{d)}\;& t:x\mapsto (2x-1)^2+(2x+1)^2 &
    \textbf{e)}\;& w:x\mapsto \frac{1}{(x+2)^3} &
    \textbf{f)}\;& z:x\mapsto \frac{x^4}{1+x^2}
  \end{align*}
\end{exo}

\begin{exo}[$\star\star\star$]
  Pour chacune des fonctions suivantes, donner l'expression de la dérivée.
  \begin{align*}
    \textbf{a)}\;& f:x\mapsto \sqrt{3x-2}\sqrt{x} &
    \textbf{b)}\;& g:x\mapsto \frac{(x+2)^3}{x+5} &
    \textbf{c)}\;& h:x\mapsto 2(5x-4)^3-\frac{1}{(5x-4)^2} \\
    \textbf{d)}\;& t:x\mapsto \sqrt{7-4x}(5-3x)^2 &
    \textbf{e)}\;& w:x\mapsto \frac{\sqrt{10x-6}}{x^2+1} &
    \textbf{f)}\;& z:x\mapsto \frac{\sqrt x}{(7x-3)^3} \\
  \end{align*}
\end{exo}

\vspace{2cm}
\setcounter{exo}{0}

\begin{exo}[Produits]
  Pour chacune des fonctions suivantes, donner l'expression de la dérivée.
  \begin{align*}
    \textbf{a)}\;& f:x\mapsto (x-1)\sqrt x &
    \textbf{b)}\;& g:x\mapsto (x^2-x)\left( 1+\frac{1}{x^2} \right) &
    \textbf{c)}\;& h:x\mapsto (\sqrt x + x^2)\left( \frac{1}{x}+\frac{1}{x^2} \right)
  \end{align*}
\end{exo}

\begin{exo}[Quotients]
  Pour chacune des fonctions suivantes, donner l'expression de la dérivée.
  \begin{align*}
    \textbf{a)}\;& f:x\mapsto \frac{1+x^4}{x+1} &
    \textbf{b)}\;& g:x\mapsto \frac{1-x}{1+\sqrt x} &
    \textbf{c)}\;& h:x\mapsto \frac{1-x^3}{1-x}
  \end{align*}
\end{exo}

\begin{exo}[Compositions]
  Pour chacune des fonctions suivantes, donner l'expression de la dérivée.
  \begin{align*}
    \textbf{a)}\;& f:x\mapsto \sqrt{2x+1} &
    \textbf{b)}\;& g:x\mapsto (5x+1)^{11} &
    \textbf{c)}\;& h:x\mapsto \frac{1}{(3x+2)^7}
  \end{align*}
\end{exo}

\begin{exo}[Un peu de tout, $\star$]
  Pour chacune des fonctions suivantes, donner l'expression de la dérivée.
  \begin{align*}
    \textbf{a)}\;& f:x\mapsto 2x^3\sqrt{x} &
    \textbf{b)}\;& g:x\mapsto 3(3x+3)^3+3 &
    \textbf{c)}\;& h:x\mapsto 3(3x^3+3)+3 \\
    \textbf{d)}\;& t:x\mapsto (2x-1)^2+(2x+1)^2 &
    \textbf{e)}\;& w:x\mapsto \frac{1}{(x+2)^3} &
    \textbf{f)}\;& z:x\mapsto \frac{x^4}{1+x^2}
  \end{align*}
\end{exo}

\begin{exo}[$\star\star\star$]
  Pour chacune des fonctions suivantes, donner l'expression de la dérivée.
  \begin{align*}
    \textbf{a)}\;& f:x\mapsto \sqrt{3x-2}\sqrt{x} &
    \textbf{b)}\;& g:x\mapsto \frac{(x+2)^3}{x+5} &
    \textbf{c)}\;& h:x\mapsto 2(5x-4)^3-\frac{1}{(5x-4)^2} \\
    \textbf{d)}\;& t:x\mapsto \sqrt{7-4x}(5-3x)^2 &
    \textbf{e)}\;& w:x\mapsto \frac{\sqrt{10x-6}}{x^2+1} &
    \textbf{f)}\;& z:x\mapsto \frac{\sqrt x}{(7x-3)^3} \\
  \end{align*}
\end{exo}


\end{document}
